map/MapIAproof.v
@@ -1,25 +1,27 @@
 Require Import CRIS MemA.
 
-From CRIS.map Require Import Header MapA MapM MapI  MapIMproof MapMAproof.
+From CRIS.map Require Import Header MapA MapM MapI MapIMproof MapMAproof.
 
 Module MapIA. Section MapIA.
-  Context `{_sinvG: !sinvG Γ Σ α β τ _I _S}.
-  Context `{_mapMG: !mapMG}.
-  Context `{_mapG: !mapG}.
-  Context `{_memG: !memG}.
+  Context `{!crisG Γ Σ α β τ _I _S}.
+  Context `{!mapMG}.
+  Context `{!mapG}.
+  Context `{!memG}.
 
   Lemma ctxr (sp_s sp_mem : string → option fspec)
       (MapInSpMap : sp_incl MapAS.sp sp_s) :
     ctx_refines
       ((MapA.t sp_s) ★ (MemA.t sp_mem), (MapA.init_cond ∗ MapM.init_cond)%I)
-      ((MapI.t)           ★ (MemA.t sp_mem), emp%I).
+      ((MapI.t)      ★ (MemA.t sp_mem), emp%I).
   Proof.
     etrans; cycle 1.
     { eapply MapIM.ctxr.
       instantiate (1:= to_sp MapMS.sp).
       i. split; try refl. unfold MapMS.sp. unseal CRIS. prove_nodup.
+      i. unfold to_sp, MapMS.sp in *; rewrite H2; ss.
     }
     eapply ctxr_frameR. rewrite -(hmod_addc_empty_l (MapM.t _)). eapply ctxr_cond_frameR.
-    eapply MapMA.ctxr; eauto. rewrite /MapMS.sp; unseal CRIS; prove_nodup. ss.
+    eapply MapMA.ctxr; eauto. unfold MapMS.sp. unseal CRIS. prove_nodup.
+    i. unfold to_sp, MapMS.sp in *; rewrite H2; ss.
   Qed.
 End MapIA. End MapIA.
